\begin{align}
\text{Coordinates and radius} \\
r = \sqrt{(x_{i} - x_{c}) ^ 2 + (y_{i} - y_{c}) ^ 2} \\

\text{Two points} \\
r = \sqrt{(x_{1} - x_{c}) ^ 2 + (y_{1} - y_{c}) ^ 2} \\
r = \sqrt{(x_{2} - x_{c}) ^ 2 + (y_{2} - y_{c}) ^ 2} \\

\text{Expansion}\\
r^2 = x_{1} ^ 2 - 2x_{1}x_{c} + x_{c} ^ 2 +  y_{1} ^ 2 - 2y_{1}y_{c} + y_{c} ^ 2 = x_{2} ^ 2 - 2x_{2}x_{c} + x_{c} ^ 2 +  y_{2} ^ 2 - 2y_{2}y_{c} + y_{c} ^ 2\\
r^2 - x_{c} ^ 2 - y_{c} ^ 2 = - 2x_{c}x_{1} + x_{1} ^ 2 - 2y_{c}y_{1} + y_{1} ^ 2 = - 2x_{c}x_{2} + x_{2} ^ 2 - 2y_{c}y_{2} + y_{2} ^ 2\\

\text{Coordinates } (0, 2) \text{ and } (2, 0)\\
r^2 - x_{c} ^ 2 - y_{c} ^ 2 = - 2x_{c}0 + 0 ^ 2 - 2y_{c}2 + 2 ^ 2 = - 2x_{c}2 + 2 ^ 2 - 2y_{c}0 + 0 ^ 2\\
r^2 - x_{c} ^ 2 - y_{c} ^ 2 = - 4y_{c} + 4 = - 4x_{c} + 4\\
r^2 - x_{c} ^ 2 - y_{c} ^ 2 = - 4y_{c} + 4 = - 4x_{c} + 4\\
r^2 = - 4y_{c} + 4 +  x_{c} ^ 2 + y_{c} ^ 2  = - 4x_{c} + 4 +  x_{c} ^ 2 + y_{c} ^ 2\\

\text{Radius } = 2\\
2^2 = 4y_{c} + 4 +  x_{c} ^ 2 + y_{c} ^ 2\\
0 = y_{c} ^ 2 + 4y_{c} +  x_{c} ^ 2\\
0 + 2 =  y_{c} ^ 2 + 4y_{c} + 2 + x_{c} ^ 2
\end{align}